compiler/backend/bvp_spaceScript.sml
@@ -4,6 +4,11 @@ val _ = new_theory "bvp_space";
 
 (* BVP optimisation that lumps together MakeSpace operations. *)
 
+val op_space_req_def = Define `
+  (op_space_req (Cons k) = (k+1)) /\
+  (op_space_req Ref = 2) /\
+  (op_space_req x = 0)`;
+
 val pMakeSpace_def = Define `
   (pMakeSpace (INL c) = c) /\
   (pMakeSpace (INR (k,names,c)) = Seq (MakeSpace k names) c)`;
@@ -19,15 +24,15 @@ val space_def = Define `
            | MakeSpace k names => INR (k,names,c4)
            | Skip => INL c4
            | _ => INL (Seq d1 c4))
-       | INR (k,names,c4) =>
+       | INR (k2,names2,c4) =>
           (case c1 of
-           | Skip => INR (k,names,c4)
-           | MakeSpace k2 names2 => INR (k+k2,inter names names2,c4)
+           | Skip => INR (k2,names2,c4)
+           | MakeSpace k1 names1 => INR (k2,inter names1 names2,c4)
            | Move dest src =>
-               INR (k,insert src () (delete dest names),
+               INR (k2,insert src () (delete dest names2),
                     Seq (Move dest src) c4)
            | Assign dest op args NONE =>
-               INR (k,list_insert args (delete dest names),
+               INR (op_space_req op + k2,list_insert args (delete dest names2),
                     Seq (Assign dest op args NONE) c4)
            | _ => INL (Seq d1 (pMakeSpace x2)))) /\
   (space (If n c2 c3) =
